implementation stream

src/tls/AEAD.fsti
@@ -83,48 +83,22 @@ type entry (i:I.id) (u:info i) =
     nonce: nonce i ->
     ad: adata ->
     #l: plainLen ->
-//    #u: info i ->
     p: plain u l ->
     c: cipher i l ->
     entry i u
 
-(*
-inline_for_extraction
-val entry : #i:I.id -> u:info i -> Type0
+
+val aead_writer: i:I.id -> Type0
+val aead_reader: #i:I.id -> w:aead_writer i -> Type0
+
+val wgetinfo: #i:I.id -> aead_writer i -> Tot (info i)
+val rgetinfo: #i:I.id -> #w:aead_writer i -> aead_reader w -> Tot (u:info i{u == wgetinfo w})
 
 
-val mk_entry (#i:I.id) (u:info i):
-    nonce:nonce i ->
-    ad:adata ->
-    #l:plainLen ->
-    p:plain u l ->
-    c:cipher i (length (as_bytes p)) ->
-    entry u
+val wlog: #i:safeid -> w:aead_writer i -> mem -> GTot (Seq.seq (entry i (wgetinfo w)))
 
-val entry_injective (#i:I.id) (u:info i)
-                    (n:nonce i) (n':nonce i)
-                    (ad:adata) (ad':adata)
-                    (#l:plainLen) (#l':plainLen)
-                    (p:plain u l) (p':plain u l')
-                    (c:cipher i l) (c':cipher i l')
-  : Lemma (let e  = mk_entry u n ad p c in
-           let e' = mk_entry u n' ad' p' c' in
-           (e == e' <==> (n == n' /\ ad == ad' /\ l == l' /\ p == p' /\ c == c')))
-
-val nonce_of_entry (#i:_) (#u:info i) (e:entry u) : nonce i
-
-val ad_of_entry (#i:_) (#u:info i) (e:entry u) : adata
-
-val plain_of_entry (#i:_) (#u:info i) (e:entry u) : (l:plainLen & p:plain u l)
-
-val cipher_of_entry (#i:_) (#u:info i) (e:entry u) : cipher u
-*)
-
-val aead_state: i:I.id -> I.rw -> Type0
-
-val getinfo: #i:I.id -> #rw:I.rw -> aead_state i rw -> Tot (info i)
-
-val log: #i:I.id -> #rw:_ -> s:aead_state i rw{safeMac i} -> mem -> GTot (Seq.seq (entry i (getinfo s)))
+let rlog (#i:safeid) (#w: aead_writer i) (r:aead_reader w) (h:mem) =
+  wlog w h
 
 let address = nat
 
@@ -143,65 +117,70 @@ let fresh_addresses (rid:rid) (addrs:Set.set address) (m0:mem) (m1:mem) =
 val shared_footprint: rset
 
 (** Downward closure of [log_region i] *)
-val footprint: #i:I.id -> #rw:_ -> aead_state i rw -> 
-  GTot (s:rset{s `Set.disjoint` shared_footprint})
+val wfootprint: #i:I.id -> aead_writer i -> 
+  GTot (s:rset{Set.disjoint s shared_footprint})
+
+(* A reader never writes to the log_region, but may write to the prf_region *)
+let rfootprint (#i:I.id) (#w:aead_writer i) (r:aead_reader w) : GTot rset =
+  assume false;
+  Set.singleton (wgetinfo w).prf_rgn
+  
+
+//  TSet.filter (fun (r:HS.rid) -> r == prf_region wr)
+//                    (footprint wr)
+
 
 //Leaving this abstract for now; but it should imply Crypto.AEAD.Invariant.safelen i len (otp_offset i)
 val safelen: I.id -> nat -> GTot bool
 
 let ok_plain_len_32 (i:I.id) = l:U32.t{safelen i (v l)}
 
-val invariant : #i:I.id -> #rw:I.rw -> aead_state i rw -> mem -> Type0
+val winvariant : #i:I.id -> aead_writer i -> mem -> Type0
+//let rinvariant (#i:I.id) (#w:aead_writer i) (r:aead_reader w) (h:mem) =
+//  winvariant w h
 
-val frame_invariant: #i:I.id -> #rw:I.rw -> s:aead_state i rw -> h0:mem -> r:rid -> h1:mem ->
-    Lemma (requires (invariant s h0 /\
-           modifies_one r h0 h1 /\
-           ~(r `Set.mem` footprint s) /\
-           ~(r `Set.mem` shared_footprint)))
-          (ensures invariant s h1)
+val wframe_invariant: #i:I.id -> w:aead_writer i -> h0:mem -> ri:rid -> h1:mem ->
+  Lemma
+    (requires (winvariant w h0 /\
+      modifies_one ri h0 h1 /\
+      ~(Set.mem ri (wfootprint w)) /\
+      ~(Set.mem ri shared_footprint)))
+    (ensures winvariant w h1)
 
-val frame_log: #i:I.id -> #rw:I.rw -> s:aead_state i rw -> l:Seq.seq (entry i (getinfo s)) ->
-  h0:mem -> r:rid -> h1:mem ->
-  Lemma (requires
-          safeMac i /\
-          log s h0 == l /\
-          modifies_one r h0 h1 /\
-          ~(r `Set.mem` footprint s))
-        (ensures log s h1 == l)
+val frame_log: #i:I.id -> w:aead_writer i -> l:Seq.seq (entry i (wgetinfo w)) ->
+  h0:mem -> ri:rid -> h1:mem ->
+  Lemma
+    (requires
+      safeId i /\
+      wlog w h0 == l /\
+      modifies_one ri h0 h1 /\
+      ~(Set.mem ri (wfootprint w)))
+    (ensures wlog w h1 == l)
 
 (*** The main stateful API ***)
 
 (** Allocating a writer **)
-val gen (i:I.id) (u:info i) : ST (aead_state i I.Writer)
-  (requires (fun h -> u.prf_rgn `disjoint` u.log_rgn))
-  (ensures  (fun h0 s h1 ->
-    getinfo s == u /\
+val gen (i:I.id) (u:info i) : ST (aead_writer i)
+  (requires (fun h -> disjoint u.prf_rgn u.log_rgn))
+  (ensures  (fun h0 w h1 ->
+    wgetinfo w == u /\
     modifies_none h0 h1 /\ // allocates only
     (exists fresh.
       fresh_addresses u.prf_rgn fresh h0 h1 /\
-      footprint s == Set.singleton u.log_rgn /\
+      wfootprint w == Set.singleton u.log_rgn /\
       shared_footprint == Set.singleton u.prf_rgn) /\
-      (safeId i ==> log s h1 == Seq.empty) /\
-        invariant s h1
+      (safeId i ==> wlog w h1 == Seq.empty) /\
+        winvariant w h1
       ))
 
 (** Building a reader from a writer **)
 
-(* A reader never writes to the log_region, but may write to the prf_region *)
-let reader_footprint (#i:I.id) (w:(aead_state i I.Writer)) : GTot rset =
-  assume false;
-  Set.singleton (getinfo w).prf_rgn
-  
-//  TSet.filter (fun (r:HS.rid) -> r == prf_region wr)
-//                    (footprint wr)
 
-val genReader (#i: I.id) (w: aead_state i I.Writer) : ST (aead_state i I.Reader)
-  (requires (fun h -> invariant w h))
+val genReader (#i: I.id) (w: aead_writer i) : ST (aead_reader w)
+  (requires (fun h -> winvariant w h))
   (ensures  (fun h0 r h1 ->
-    HS.modifies Set.empty h0 h1 /\
-    invariant r h1 /\
-    getinfo r == getinfo w /\
-    footprint r == reader_footprint w)
+    modifies Set.empty h0 h1 /\
+    winvariant w h1)
   )
 
 (*
@@ -276,13 +255,13 @@ let entry_of
   mk_entry n aad p c
 *)
 
-let entry_for_nonce (#i:I.id) (#rw:I.rw) (n:nonce i) (s:aead_state i rw) (h:mem)
-  : Ghost (option (entry i (getinfo s))) (requires safeId i) (ensures fun _ -> True) =
-  Seq.find_l (fun e -> Entry?.nonce e = n) (log s h)
+let wentry_for_nonce (#i:I.id) (n:nonce i) (w:aead_writer i) (h:mem)
+  : Ghost (option (entry i (wgetinfo w))) (requires safeId i) (ensures fun _ -> True) =
+  Seq.find_l (fun e -> Entry?.nonce e = n) (wlog w h)
 
-let fresh_nonce (#i:I.id) (#rw:I.rw) (n:nonce i) (s:aead_state i rw) (h:mem)
+let fresh_nonce (#i:I.id) (n:nonce i) (s:aead_writer i) (h:mem)
   : Ghost bool (requires safeId i) (ensures fun _ -> True) =
-  None? (entry_for_nonce n s h)
+  None? (wentry_for_nonce n s h)
 
 (*let just_one_buffer (#a:Type) (b:Buffer.buffer a) : GTot fp =
    as_set [(Buffer.frameOf b, SomeRefs (as_set [Buffer.as_addr b]))]
@@ -290,39 +269,37 @@ let fresh_nonce (#i:I.id) (#rw:I.rw) (n:nonce i) (s:aead_state i rw) (h:mem)
 
 val encrypt
   (i: I.id)
-  (w: aead_state i I.Writer)
+  (w: aead_writer i)
   (n: iv (I.cipherAlg_of_id i))
   (aad: adata)
   (l: plainLen)
-  (p: plain (getinfo w) l)
+  (p: plain (wgetinfo w) l)
   : ST (cipher i l)
   (requires (fun h0 ->
-//    enc_dec_separation st aad plain cipher_tag /\
-//    enc_dec_liveness st aad plain cipher_tag h /\
-    invariant w h0 /\
+    winvariant w h0 /\
     (safeId i ==> fresh_nonce n w h0)))
   (ensures (fun h0 c h1 ->
-    modifies (Set.union (footprint w) shared_footprint) h0 h1 /\
-//    enc_dec_liveness st aad plain cipher_tag h1 /\
-    invariant w h1 /\
+    modifies (Set.union (wfootprint w) shared_footprint) h0 h1 /\
+    winvariant w h1 /\
     (safeId i ==>
-      log w h1 == Seq.snoc (log w h0) (Entry n aad p c))))
+      wlog w h1 == Seq.snoc (wlog w h0) (Entry n aad p c))))
 
 val decrypt
   (i: I.id)
-  (r: aead_state i I.Reader)
+  (#w: aead_writer i)
+  (r: aead_reader w)
   (aad:adata)
   (n: iv (I.cipherAlg_of_id i))
   (l:plainLen)
   (c:cipher i l)
-  : ST (option (plain (getinfo r) l))
+  : ST (option (plain (rgetinfo r) l))
   (requires (fun h0 ->
-    invariant r h0))
+    winvariant w h0))
   (ensures fun h0 res h1 ->
-    invariant r h1 /\
-    modifies (Set.union (footprint r) shared_footprint) h0 h1 /\
+    winvariant w h1 /\
+    modifies (Set.union (rfootprint r) shared_footprint) h0 h1 /\
     (safeId i ==>
-      (match entry_for_nonce n r h0 with
+      (match wentry_for_nonce n w h0 with
       | None -> None? res
       | Some (Entry _ aad' #l' p' c') ->
         (if aad' = aad && c' = c && l = l' then res = Some p'
